Continuing local roots

theories/interop/basics.v
@@ -168,6 +168,8 @@ Implicit Type θ : addr_map.
    and keeping alive *)
 Notation roots_map := (gmap addr lval).
 
+Definition roots_dom (roots : list roots_map) :=
+  List.fold_left (fun acc r => acc ∪ (dom r)) roots ∅.
 
 (** lloc_map injectivity: lloc_maps are always injective wrt public locs and
    foreign ids
@@ -271,24 +273,25 @@ Inductive repr_lval : addr_map → lval → C_intf.val → Prop :=
     θ !! γ = Some a →
     repr_lval θ (Lloc γ) (C_intf.LitV (C_intf.LitLoc a)).
 
-Inductive repr_roots : addr_map → memory → roots_map → Prop :=
+Inductive repr_roots : addr_map → memory → list roots_map → Prop :=
   | repr_roots_emp θ :
-    repr_roots θ ∅ ∅
-  | repr_roots_elem θ a v w roots mem :
-    repr_roots θ mem roots →
+    repr_roots θ ∅ [∅]
+  | repr_roots_push θ mem roots :
+    repr_roots θ mem roots → repr_roots θ mem (∅ :: roots)
+  | repr_roots_extend θ a v w roots_hd roots_tl mem :
+    repr_roots θ mem (roots_hd :: roots_tl) →
     repr_lval θ v w →
-    a ∉ dom roots →
-    a ∉ dom (mem) →
-    repr_roots θ (<[ a := Storing w ]> mem) (<[ a := v ]> roots).
+    a ∉ dom mem →
+    Forall (λ roots, a ∉ dom roots) (roots_hd :: roots_tl) →
+    repr_roots θ (<[ a := Storing w ]> mem) (<[ a := v ]> roots_hd :: roots_tl).
 
 Definition repr_raw (θ : addr_map) (roots : list roots_map) (privmem mem memr : memory) : Prop :=
-  Forall (repr_roots θ memr) roots  ∧
+  repr_roots θ memr roots ∧
   privmem ##ₘ memr ∧
   mem = memr ∪ privmem.
 
 Definition repr (θ : addr_map) (roots : list roots_map) (privmem mem : memory) : Prop :=
   ∃ memr, repr_raw θ roots privmem mem memr.
-
 
 (** Block-level representation of ML values and store *)
 Inductive is_val : lloc_map → lstore → val → lval → Prop :=
@@ -1044,12 +1047,14 @@ Proof.
   eapply H2; eauto. by constructor.
 Qed.
 
-Lemma repr_roots_dom θ a b : repr_roots θ a b -> dom a = dom b.
+Lemma repr_roots_dom θ a b :
+  repr_roots θ a b -> dom a = roots_dom b.
 Proof.
-  induction 1.
-  + by do 2 rewrite dom_empty_L.
-  + by do 2 rewrite dom_insert_L; rewrite IHrepr_roots.
-Qed.
+Admitted.
+(*   induction 1. *)
+(*   + by do 2 rewrite dom_empty_L. *)
+(*   + by do 2 rewrite dom_insert_L; rewrite IHrepr_roots. *)
+(* Qed. *)
 
 Lemma code_int_inj z1 z2 : code_int z1 = code_int z2 → z1 = z2.
 Proof.
