theories/interop/gctoken.v
@@ -56,16 +56,16 @@ Context `{!wrapperGCtokG Σ}.
 
 Definition GC (θ : addr_map) : iProp Σ :=
   ∃ (ζ : lstore) (χ : lloc_map) (σMLvirt : store)
-    (roots_s : gset addr) (roots_m : gmap addr lval),
+    (roots_s : gset addr) (roots_m : list roots_map),
     "GCζ" ∷ ghost_var wrapperG_γζ (1/2) ζ
   ∗ "GCχ" ∷ ghost_var wrapperG_γχ (1/2) χ
   ∗ "GCθ" ∷ ghost_var wrapperG_γθ (1/2) θ
   ∗ "GCHGH" ∷ HGH χ (Some σMLvirt) ζ
   ∗ "GCinit" ∷ ghost_var wrapperG_γat_init (1/2) false
   ∗ "GCroots" ∷ ghost_var wrapperG_γroots_set (1/2) roots_s
-  ∗ "GCrootsm" ∷ ghost_map_auth wrapperG_γroots_map 1 roots_m
-  ∗ "GCrootspto" ∷ ([∗ map] a ↦ v ∈ roots_m, ∃ w, a ↦C w ∗ ⌜repr_lval θ v w⌝)
-  ∗ "%Hrootsdom" ∷ ⌜dom roots_m = roots_s⌝
+  ∗ "GCrootsm" ∷ [∗ list] roots ∈ roots_m, ghost_map_auth wrapperG_γroots_map 1 roots
+  ∗ "GCrootspto" ∷ [∗ list] roots ∈ roots_m, ([∗ map] a ↦ v ∈ roots, ∃ w, a ↦C w ∗ ⌜repr_lval θ v w⌝)
+  ∗ "%Hrootsdom" ∷ ⌜roots_dom roots_m = roots_s⌝
   ∗ "%Hrootslive" ∷ ⌜roots_are_live θ roots_m⌝
   ∗ "%HGCOK" ∷ ⌜GC_correct ζ θ⌝.
 
